Fix a reifier to support free array variables

Examples/max_idx2.v
@@ -2,19 +2,11 @@ Require Import Monad SkelLib Computation ZArith TypedTerm Program.
 Open Scope Z_scope.
 
 Definition max_idx (arr : list Z) : comp (list (Z * Z)) :=
-  reduceM (fun x y => if (fst x) <? (fst y) then ret x else ret y) (zip arr (seq 0 (length arr))).
+  reduceM (fun x y => if (fst x) <? (fst y) then ret x else ret y) (zip arr (seq 0 (len arr))).
 
-Lemma gen_seq st len : ret (seq st len) = gen (fun x => ret (st + x)) (Z.of_nat len).
-Proof.
-Admitted.  
-
-Lemma zip_seq (a1 a2 : list Z) :
-  gen (fun i =>
-         do! t1 := nth_error a1 i in
-         do! t2 := nth_error a2 i in
-         ret (t1, t2)) (Z.min (Z.of_nat (length a1)) (Z.of_nat (length a2))) = 
-  ret (zip a1 a2).
-Admitted. 
+Lemma zip_seq (arr : list Z) : ret (zip arr (seq 0 (len arr))) =
+                               gen (fun i => do! x := nth_error arr i in ret (x, i)) (len arr).
+Admitted.
 
 Definition max_idx_IR:  {p : Skel.AS (Skel.TZ :: nil) (Skel.TTup Skel.TZ Skel.TZ) |
       equiv1 p (max_idx)}.
@@ -28,23 +20,26 @@ Proof.
   lazymatch goal with
   | [|- _ = do! t := ?ae in @?res t] => pose ae
   end.
-  cutrewrite (ret (zip x0 (seq 0 (length x0))) =
-              (do! t := ret (seq 0 (length x0)) in ret (zip x0 t) : comp _)); [|eauto].
+  rewrite (zip_seq x0).
+  (* cutrewrite (ret (zip x0 (seq 0 (len x0))) = *)
+  (*             (do! t := ret (seq 0 (len x0)) in ret (zip x0 t) : comp _)); [|eauto]. *)
 
-  repeat lazymatch goal with
-  | [|- context [do! t := do! u := ret ?ae in @?f u in @?g t]] => 
-    let t := eval cbv beta in (do! t := do! u := ret ae in f u in g t) in 
-    cutrewrite (t = (do! u := ret ae in do! t := f u in g t)); [|eauto]
-  end.
+  (* repeat lazymatch goal with *)
+  (* | [|- context [do! t := do! u := ret ?ae in @?f u in @?g t]] =>  *)
+  (*   let t := eval cbv beta in (do! t := do! u := ret ae in f u in g t) in  *)
+  (*   cutrewrite (t = (do! u := ret ae in do! t := f u in g t)); [|eauto] *)
+  (* end. *)
+
+  Lemma ret_id (A : Type) (t : comp A) : t = (do! x := t in ret x).
+  Proof.
+    cbv; destruct t; eauto.
+  Qed.
 
   lazymatch goal with
   | [|- _ = ?term ] =>
-    idtac term;
-    bind_last (fun _ : unit => term) ltac:(fun t =>
-      let t := eval_tup (t tt) in
-      cutrewrite (term = t)); [|dest; eauto]
+    cutrewrite (term = do! x := term in ret x); [|apply ret_id]
   end.
-
+  
   reflexivity.
 
   apply H.
@@ -57,8 +52,9 @@ Proof.
 
   unfold equiv1; simpl; intros; auto.
   unfold ret, bind; simpl.
-  rewrite Nat2Z.id.
   f_equal. f_equal.
+  repeat (let t := fresh "t" in extensionality t).
+  f_equal.
   repeat (let t := fresh "t" in extensionality t).
   destruct (_ <? _); auto.
 Defined.
@@ -71,7 +67,7 @@ Definition max_idx_CUDA : Host.Prog :=
     Compiler.compile_prog 1024 24 ir
   end.
 
-Definition res := save_to_file max_idx_CUDA "max_idx.cu".
+Definition res := save_to_file max_idx_CUDA "max_idx_opt.cu".
 
 Cd "extracted".
 
